<?xml version="1.0"?>
<rdf:RDF xmlns="https://data.istex.fr/ontology/istex#"
     xml:base="https://data.istex.fr/ontology/istex"
     xmlns:schema="http://schema.org/"
     xmlns:ns="http://www.w3.org/2003/06/sw-vocab-status/ns#"
     xmlns:owl="http://www.w3.org/2002/07/owl#"
     xmlns:xsd="http://www.w3.org/2001/XMLSchema#"
     xmlns:skos="http://www.w3.org/2004/02/skos/core#"
     xmlns:rdfs="http://www.w3.org/2000/01/rdf-schema#"
     xmlns:rdf="http://www.w3.org/1999/02/22-rdf-syntax-ns#"
     xmlns:terms="http://purl.org/dc/terms/"
     xmlns:xml="http://www.w3.org/XML/1998/namespace"
     xmlns:dcat="http://www.w3.org/ns/dcat#"
     xmlns:vann="http://purl.org/vocab/vann/"
     xmlns:prov="http://www.w3.org/ns/prov#"
     xmlns:wot="http://xmlns.com/wot/0.1/"
     xmlns:foaf="http://xmlns.com/foaf/0.1/"
     xmlns:dc="http://purl.org/dc/elements/1.1/"
     xmlns:cc="http://creativecommons.org/ns#"
     xmlns:voaf="http://purl.org/vocommons/voaf#"
     xmlns:vs="http://www.w3.org/2003/06/sw-vocab-status/ns#">
    <owl:Ontology rdf:about="https://data.istex.fr/ontology/istex#">
        <rdf:type rdf:resource="https://data.istex.fr/ontology/istex#Vocabulary"/>
        <vann:preferredNamespacePrefix>istex</vann:preferredNamespacePrefix>
        <vann:preferredNamespaceUri>https://data.istex.fr/ontology/istex#</vann:preferredNamespaceUri>
        <owl:imports rdf:resource="http://www.w3.org/ns/dcat"/>
        <owl:imports rdf:resource="http://purl.org/ontology/bibo/"/>
        <owl:imports rdf:resource="http://www.w3.org/ns/prov-o-20130430"/>
        <owl:imports rdf:resource="http://www.w3.org/2004/02/skos/core"/>
        <owl:imports rdf:resource="http://xmlns.com/foaf/0.1/"/>
    </owl:Ontology>
    
    <owl:Ontology rdf:about="https://data.istex.fr/ontology/istex#">
        <dc:title xml:lang="en">Vocabulary of ISTEX project</dc:title>
        <dc:description xml:lang="en">A vocabulary to describe ISTEX' linked data vocabularies and their relations.</dc:description>
        <rdfs:label xml:lang="fr">Ontologie du projet ISTEX</rdfs:label>
    </owl:Ontology>
    
    <owl:Ontology rdf:about="https://data.istex.fr/ontology/istex#">
        <dc:issued rdf:datatype="http://www.w3.org/2001/XMLSchema#date">2017-04-11</dc:issued>
        <dc:modified rdf:datatype="http://www.w3.org/2001/XMLSchema#date">2019-05-16</dc:modified>
        <owl:versionInfo rdf:datatype="http://www.w3.org/2001/XMLSchema#decimal">2.0</owl:versionInfo>
        <owl:versionIRI rdf:resource="https://data.istex.fr/ontology/istex"/>
        <rdfs:comment xml:lang="fr">v 2.0 16-05-2019 Ajouts des recommandations du Linked Open Vocabularies (LOV)

v 1.9 17-12-2018 Ajout de la propriété istex:eISBN

v 1.8 11-10-2018 Ajout de la propriété istex:publicationTitle
Suppression de la propriété istex:bookTitle
Suppression de la propriété istex:databaseTitle
Suppression de la propriété istex:journalTitle
Suppression de la propriété istex:referenceWorksTitle
Suppression de la propriété istex:seriesTitle

v 1.7 21-09-2018 Ajout de la propriété istex:bookTitle
Ajout de la propriété istex:databaseTitle
Ajout de la propriété istex:journalTitle
Ajout de la propriété istex:referenceWorksTitle
Ajout de la propriété istex:seriesTitle

v 1.6.1 22-05-2018 Ajout de la propriété istex:analysisType
Ajout de la propriété istex:addresseeWork

v 1.6 30-01-2018 Ajout de la propriété istex:tool

v 1.5 22-12-2017 Ajout de la propriété istex:subjectScopus
Ajout de la classe istex:ScopusConcept

v 1.4 16-10-2017 Ajout de la propriété istex:identityProvider
Suppression de istex:catalog
Suppression de istex:SoftwareApplication
Ajout commentaires niveau Classe et Object Properties
Ajout de la classe istex:NamedEntityConcept
Ajout de la classe istex:EnrichmentProcessConcept
Ajout de l'object property istex:enrichmentProcess

V 1.3 22-09-2017 Ajout de la propriété istex:accessURL
Ajout de la propriété istex:subjectLabel
Ajout de la propriété istex:catalog
Ajout de la Classe istex:SoftwareApplication + ajout range à istex:enrichmentType et istex:constraint
Ajout de la Classe istex:PublisherConcept
Suppression domaine istex:query + ajout range xsd:anyURI au lieu de rdfs:literal

V 1.2 22-06-2017 Changement uri pour passer à https://data.istex.fr/ontology/istex
Ajouté la propriété istex:query
Ajouté les propriétés  schema:endDate et schema:startDate ainsi que la classe dct:PeriodOfTime et la propriété dct:temporal pour décrire la période de couverture des lots de chargement
Ajouté la propriété istex:affiliation (existe dans MODS XML mais pas dans MODS OWL)
Ajouté la propriété quantityOfItems pour décrire le nombre de titres présents dans chaque corpus ISTEX

V 1.1 12-04-2017 Ajout de la classe dcterms:LinguisticSystem - les valeurs de dcterms:language sont des instances de la classe LinguisticSystem

V 1.0 11-04-2017 Première version de l'ontologie basée sur bibo, skos et prov-o</rdfs:comment>
    </owl:Ontology>
    
    <owl:Ontology rdf:about="https://data.istex.fr/ontology/istex#">
        <dc:rights>All rights reserved. Licence Etalab</dc:rights>
        <dc:license rdf:resource="https://www.etalab.gouv.fr/licence-ouverte-open-licence"/>
        <dc:contributor>
            <foaf:Person>
                <foaf:name>Stephanie GREGORIO</foaf:name>
                <foaf:givenName>Stephanie</foaf:givenName>
                <foaf:familyName>Gregorio</foaf:familyName>
                <foaf:mbox rdf:resource="mailto:stephanie.gregorio@inist.fr"/>
            </foaf:Person>
        </dc:contributor>
        <dc:contributor>
            <foaf:Person>
                <foaf:name>François PARMENTIER</foaf:name>
                <foaf:givenName>François</foaf:givenName>
                <foaf:familyName>Parmentier</foaf:familyName>
                <foaf:mbox rdf:resource="mailto:françois.parmentier@inist.fr"/>
            </foaf:Person>
        </dc:contributor>
        <dc:creator>
            <foaf:Organization rdf:about="http://dbpedia.org/resource/Institut_de_l%27information_scientifique_et_technique"/>
        </dc:creator>
        <dc:publisher>
            <foaf:Organization rdf:about="https://www.istex.fr/"/>
        </dc:publisher> 
    </owl:Ontology>
    


    <!-- 
    ///////////////////////////////////////////////////////////////////////////////////////
    //
    // Object Properties
    //
    ///////////////////////////////////////////////////////////////////////////////////////
     -->

    


    <!-- http://purl.org/dc/terms/language -->

    <owl:ObjectProperty rdf:about="http://purl.org/dc/terms/language"/>
    


    <!-- http://purl.org/dc/terms/requires -->

    <owl:ObjectProperty rdf:about="http://purl.org/dc/terms/requires"/>
    


    <!-- http://purl.org/dc/terms/type -->

    <owl:ObjectProperty rdf:about="http://purl.org/dc/terms/type">
        <rdfs:comment xml:lang="en">Recommended best practice is to use a controlled vocabulary such as the DCMI Type Vocabulary [DCMITYPE]. To describe the file format, physical medium, or dimensions of the resource, use the Format element. The nature or genre of the resource.</rdfs:comment>
        <rdfs:label xml:lang="en">type</rdfs:label>
    </owl:ObjectProperty>
    


    <!-- https://data.istex.fr/ontology/istex#contentType -->

    <owl:ObjectProperty rdf:about="https://data.istex.fr/ontology/istex#contentType">
        <rdfs:domain rdf:resource="http://purl.org/ontology/bibo/Document"/>
        <rdfs:range rdf:resource="https://data.istex.fr/ontology/istex#ContentTypeConcept"/>
        <rdfs:comment xml:lang="fr">Type de contenus répertoriés dans les documents ISTEX</rdfs:comment>
        <rdfs:comment xml:lang="en">Type of content listed in ISTEX documents</rdfs:comment>
        <rdfs:label xml:lang="en">content type</rdfs:label>
        <rdfs:label xml:lang="fr">type de contenu</rdfs:label>
        <rdfs:isDefinedBy rdf:resource="https://data.istex.fr/ontology/istex#"/>
    </owl:ObjectProperty>
    


    <!-- https://data.istex.fr/ontology/istex#enrichmentProcess -->

    <owl:ObjectProperty rdf:about="https://data.istex.fr/ontology/istex#enrichmentProcess">
        <rdfs:domain rdf:resource="http://purl.org/ontology/bibo/Document"/>
        <rdfs:range rdf:resource="https://data.istex.fr/ontology/istex#EnrichmentProcessConcept"/>
        <rdfs:comment xml:lang="fr">Processus de fabrication des enrichissements</rdfs:comment>
        <rdfs:comment xml:lang="en">Process of making enrichments</rdfs:comment>
        <rdfs:label xml:lang="en">Enrichment process</rdfs:label>
        <rdfs:label xml:lang="fr">Processus d'enrichissement</rdfs:label>
        <rdfs:isDefinedBy rdf:resource="https://data.istex.fr/ontology/istex#"/>
    </owl:ObjectProperty>
    


    <!-- https://data.istex.fr/ontology/istex#extractedEntity -->

    <owl:ObjectProperty rdf:about="https://data.istex.fr/ontology/istex#extractedEntity">
        <rdfs:domain rdf:resource="http://purl.org/ontology/bibo/Document"/>
        <rdfs:range rdf:resource="http://www.w3.org/2004/02/skos/core#Concept"/>
        <rdfs:comment xml:lang="fr">Entité nommée extraite du plein texte des document ISTEX</rdfs:comment>
        <rdfs:comment xml:lang="en">Named entity extracted from full text of ISTEX documents</rdfs:comment>
        <rdfs:label xml:lang="en">Extracted entity</rdfs:label>
        <rdfs:label xml:lang="fr">Entité nommée extraite</rdfs:label>
        <rdfs:isDefinedBy rdf:resource="https://data.istex.fr/ontology/istex#"/>
    </owl:ObjectProperty>
    


    <!-- https://data.istex.fr/ontology/istex#extractedGeog -->

    <owl:ObjectProperty rdf:about="https://data.istex.fr/ontology/istex#extractedGeog">
        <rdfs:subPropertyOf rdf:resource="https://data.istex.fr/ontology/istex#extractedEntity"/>
        <rdfs:domain rdf:resource="http://purl.org/ontology/bibo/Document"/>
        <rdfs:range rdf:resource="https://data.istex.fr/ontology/istex#GeographicConcept"/>
        <rdfs:comment xml:lang="fr">Entité géographique physique extraite du plein texte des documents ISTEX</rdfs:comment>
        <rdfs:comment xml:lang="en">Physical geographic entity extracted from the full text of ISTEX documents</rdfs:comment>
        <rdfs:label xml:lang="en">extracted geographic entity</rdfs:label>
        <rdfs:label xml:lang="fr">Entité nommée geographique extraite</rdfs:label>
        <rdfs:isDefinedBy rdf:resource="https://data.istex.fr/ontology/istex#"/>
    </owl:ObjectProperty>
    


    <!-- https://data.istex.fr/ontology/istex#extractedOrganization -->

    <owl:ObjectProperty rdf:about="https://data.istex.fr/ontology/istex#extractedOrganization">
        <rdfs:subPropertyOf rdf:resource="https://data.istex.fr/ontology/istex#extractedEntity"/>
        <rdfs:domain rdf:resource="http://purl.org/ontology/bibo/Document"/>
        <rdfs:range rdf:resource="https://data.istex.fr/ontology/istex#OrganizationConcept"/>
        <rdfs:comment xml:lang="fr">Entité organisationnelle extraite du plein texte des documents ISTEX</rdfs:comment>
        <rdfs:comment xml:lang="en">Additional organizational entity of the full text of ISTEX documents</rdfs:comment>
        <rdfs:label xml:lang="en">extracted organization entity</rdfs:label>
        <rdfs:label xml:lang="fr">Entité nommée d' organisation extraite</rdfs:label>
        <rdfs:isDefinedBy rdf:resource="https://data.istex.fr/ontology/istex#"/>
    </owl:ObjectProperty>
    


    <!-- https://data.istex.fr/ontology/istex#extractedPlace -->

    <owl:ObjectProperty rdf:about="https://data.istex.fr/ontology/istex#extractedPlace">
        <rdfs:subPropertyOf rdf:resource="https://data.istex.fr/ontology/istex#extractedEntity"/>
        <rdfs:domain rdf:resource="http://purl.org/ontology/bibo/Document"/>
        <rdfs:range rdf:resource="https://data.istex.fr/ontology/istex#PlaceConcept"/>
        <rdfs:comment xml:lang="fr">Entité géographique administrative extraite du plein texte des documents ISTEX</rdfs:comment>
        <rdfs:comment xml:lang="en">Geographic administrative entity extracted from the full text of ISTEX documents</rdfs:comment>
        <rdfs:label xml:lang="en">extracted place entity</rdfs:label>
        <rdfs:label xml:lang="fr">Entité nommée de lieu extraite</rdfs:label>
        <rdfs:isDefinedBy rdf:resource="https://data.istex.fr/ontology/istex#"/>
    </owl:ObjectProperty>
    


    <!-- https://data.istex.fr/ontology/istex#publicationType -->

    <owl:ObjectProperty rdf:about="https://data.istex.fr/ontology/istex#publicationType">
        <rdfs:subPropertyOf rdf:resource="http://www.w3.org/2002/07/owl#topObjectProperty"/>
        <rdfs:domain rdf:resource="http://purl.org/ontology/bibo/Document"/>
        <rdfs:range rdf:resource="https://data.istex.fr/ontology/istex#PublicationTypeConcept"/>
        <rdfs:comment xml:lang="fr">Type de publication catégorisé dans les documents ISTEX</rdfs:comment>
        <rdfs:comment xml:lang="en">Categorized publication type in ISTEX documents</rdfs:comment>
        <rdfs:label xml:lang="en">publication type</rdfs:label>
        <rdfs:label xml:lang="fr">type de publication</rdfs:label>
        <rdfs:isDefinedBy rdf:resource="https://data.istex.fr/ontology/istex#"/>
    </owl:ObjectProperty>
    


    <!-- https://data.istex.fr/ontology/istex#subjectInist -->

    <owl:ObjectProperty rdf:about="https://data.istex.fr/ontology/istex#subjectInist">
        <rdfs:subPropertyOf rdf:resource="http://purl.org/dc/terms/subject"/>
        <rdfs:domain rdf:resource="http://purl.org/ontology/bibo/Document"/>
        <rdfs:range rdf:resource="https://data.istex.fr/ontology/istex#InistConcept"/>
        <rdfs:comment xml:lang="fr">Indique la ou les catégorie(s) Inist du document</rdfs:comment>
        <rdfs:comment xml:lang="en">Indicates the category(es) inist of the document</rdfs:comment>
        <rdfs:label xml:lang="en">Inist category</rdfs:label>
        <rdfs:label xml:lang="fr">catégorie Inist</rdfs:label>
        <rdfs:isDefinedBy rdf:resource="https://data.istex.fr/ontology/istex#"/>
    </owl:ObjectProperty>
    


    <!-- https://data.istex.fr/ontology/istex#subjectScienceMetrix -->

    <owl:ObjectProperty rdf:about="https://data.istex.fr/ontology/istex#subjectScienceMetrix">
        <rdfs:subPropertyOf rdf:resource="http://purl.org/dc/terms/subject"/>
        <rdfs:domain rdf:resource="http://purl.org/ontology/bibo/Document"/>
        <rdfs:range rdf:resource="https://data.istex.fr/ontology/istex#ScienceMetrixConcept"/>
        <rdfs:comment xml:lang="fr">Indique la ou les catégorie(s) Science Metrix du document</rdfs:comment>
        <rdfs:comment xml:lang="en">Indicates the Science Metrix category(es) of the document</rdfs:comment>
        <rdfs:label xml:lang="en">Science Metrix category</rdfs:label>
        <rdfs:label xml:lang="fr">catégorie Science Metrix</rdfs:label>
        <rdfs:isDefinedBy rdf:resource="https://data.istex.fr/ontology/istex#"/>
    </owl:ObjectProperty>
    


    <!-- https://data.istex.fr/ontology/istex#subjectWos -->

    <owl:ObjectProperty rdf:about="https://data.istex.fr/ontology/istex#subjectWos">
        <rdfs:subPropertyOf rdf:resource="http://purl.org/dc/terms/subject"/>
        <rdfs:domain rdf:resource="http://purl.org/ontology/bibo/Document"/>
        <rdfs:range rdf:resource="https://data.istex.fr/ontology/istex#WosConcept"/>
        <rdfs:comment xml:lang="fr">Indique la ou les catégorie(s) Web of Science du document</rdfs:comment>
        <rdfs:comment xml:lang="en">Indicates the category(es) Web of Science of the document</rdfs:comment>
        <rdfs:label xml:lang="en">Web of Science category</rdfs:label>
        <rdfs:label xml:lang="fr">catégorie Web of Science</rdfs:label>
        <rdfs:isDefinedBy rdf:resource="https://data.istex.fr/ontology/istex#"/>
    </owl:ObjectProperty>
    
    
     <!-- https://data.istex.fr/ontology/istex#subjectScopus -->

    <owl:ObjectProperty rdf:about="https://data.istex.fr/ontology/istex#subjectScopus">
        <rdfs:subPropertyOf rdf:resource="http://purl.org/dc/terms/subject"/>
        <rdfs:domain rdf:resource="http://purl.org/ontology/bibo/Document"/>
        <rdfs:range rdf:resource="https://data.istex.fr/ontology/istex#ScopusConcept"/>
        <rdfs:comment xml:lang="fr">Indique la ou les catégorie(s) Scopus du document</rdfs:comment>
        <rdfs:comment xml:lang="en">Indicates the Scopus category(es) of the document</rdfs:comment>
        <rdfs:label xml:lang="en">Scopus category</rdfs:label>
        <rdfs:label xml:lang="fr">catégorie Scopus</rdfs:label>
        <rdfs:isDefinedBy rdf:resource="https://data.istex.fr/ontology/istex#"/>
    </owl:ObjectProperty>
    

    <!-- 
    ///////////////////////////////////////////////////////////////////////////////////////
    //
    // Data properties
    //
    ///////////////////////////////////////////////////////////////////////////////////////
     -->

    


    <!-- http://purl.org/ontology/bibo/identifier -->

    <owl:DatatypeProperty rdf:about="http://purl.org/ontology/bibo/identifier">
        <rdfs:label>bibo:identifier</rdfs:label>
    </owl:DatatypeProperty>
    


    <!-- http://schema.org/endDate -->

    <owl:DatatypeProperty rdf:about="http://schema.org/endDate">
        <rdfs:domain rdf:resource="http://purl.org/dc/terms/PeriodOfTime"/>
        <rdfs:range rdf:resource="http://www.w3.org/2001/XMLSchema#dateTime"/>
        <rdfs:comment xml:lang="en">The end date and time of the item (in ISO 8601 date format).</rdfs:comment>
        <rdfs:label xml:lang="en">end Date</rdfs:label>
    </owl:DatatypeProperty>
    


    <!-- http://schema.org/startDate -->

    <owl:DatatypeProperty rdf:about="http://schema.org/startDate">
        <rdfs:domain rdf:resource="http://purl.org/dc/terms/PeriodOfTime"/>
        <rdfs:range rdf:resource="http://www.w3.org/2001/XMLSchema#dateTime"/>
        <rdfs:comment xml:lang="en">The start date and time of the item (in ISO 8601 date format).</rdfs:comment>
        <rdfs:label xml:lang="en">start Date</rdfs:label>
    </owl:DatatypeProperty>
    


    <!-- https://data.istex.fr/ontology/istex#accessURL -->

    <owl:DatatypeProperty rdf:about="https://data.istex.fr/ontology/istex#accessURL">
        <rdfs:domain rdf:resource="http://purl.org/ontology/bibo/Document"/>
        <rdfs:range rdf:resource="http://www.w3.org/2001/XMLSchema#anyURI"/>
        <rdfs:comment xml:lang="fr">Lien direct vers le document en format PDF</rdfs:comment>
        <rdfs:comment xml:lang="en">Direct link to the document in PDF format</rdfs:comment>
        <rdfs:label xml:lang="en">access URL</rdfs:label>
        <rdfs:label xml:lang="fr">access URL</rdfs:label>
        <rdfs:isDefinedBy rdf:resource="https://data.istex.fr/ontology/istex#"/>
    </owl:DatatypeProperty>
    
    <!-- https://data.istex.fr/ontology/istex#addresseeWork -->

    <owl:DatatypeProperty rdf:about="https://data.istex.fr/ontology/istex#accessURL">
        <rdfs:domain rdf:resource="http://xmlns.com/foaf/0.1/Agent"/>
        <rdfs:range rdf:resource="http://www.w3.org/2000/01/rdf-schema#Literal"/>
        <rdfs:comment xml:lang="fr">Organisme pour lequel est constitué le corpus</rdfs:comment>
        <rdfs:comment xml:lang="en">Organization for which the corpus is made up</rdfs:comment>
        <rdfs:label xml:lang="en">addressee Work</rdfs:label>
        <rdfs:isDefinedBy rdf:resource="https://data.istex.fr/ontology/istex#"/>
    </owl:DatatypeProperty>


    <!-- https://data.istex.fr/ontology/istex#affiliation -->

    <owl:DatatypeProperty rdf:about="https://data.istex.fr/ontology/istex#affiliation">
        <rdfs:domain rdf:resource="http://xmlns.com/foaf/0.1/Agent"/>
        <rdfs:range rdf:resource="http://www.w3.org/2000/01/rdf-schema#Literal"/>
        <rdfs:comment xml:lang="fr">Décrit une affiliation d'un ou de plusieurs auteurs (physique ou moral) du document.</rdfs:comment>
        <rdfs:comment xml:lang="en">Describes one or more authors (physical or moral) of the document.</rdfs:comment>
        <rdfs:label xml:lang="en">affiliation</rdfs:label>
        <rdfs:label xml:lang="fr">affiliation</rdfs:label>
        <rdfs:isDefinedBy rdf:resource="https://data.istex.fr/ontology/istex#"/>
    </owl:DatatypeProperty>
    
    
    <!-- https://data.istex.fr/ontology/istex#analysisType -->

    <owl:DatatypeProperty rdf:about="https://data.istex.fr/ontology/istex#analysisType">
        <rdfs:domain rdf:resource="http://www.w3.org/ns/prov#Activity"/>
        <rdfs:range rdf:resource="http://www.w3.org/2000/01/rdf-schema#Literal"/>
        <rdfs:comment xml:lang="fr">Type d’analyse réalisée sur le corpus par le destinataire</rdfs:comment>
        <rdfs:comment xml:lang="en">Type of analysis performed on the corpus by the recipient</rdfs:comment>
        <rdfs:label xml:lang="en">analysis type</rdfs:label>
        <rdfs:label xml:lang="fr">type d'analyse</rdfs:label>
        <rdfs:isDefinedBy rdf:resource="https://data.istex.fr/ontology/istex#"/>
    </owl:DatatypeProperty>
    
    
    <!-- https://data.istex.fr/ontology/istex#constraint -->

    <owl:DatatypeProperty rdf:about="https://data.istex.fr/ontology/istex#constraint">
        <rdfs:domain rdf:resource="https://data.istex.fr/ontology/istex#EnrichmentProcessConcept"/>
        <rdfs:range rdf:resource="http://www.w3.org/2000/01/rdf-schema#Literal"/>
        <rdfs:comment xml:lang="fr">Les contraintes d'utilisation du processus d'enrichissement</rdfs:comment>
        <rdfs:comment xml:lang="en">The constraints of using the enrichment process</rdfs:comment>
        <rdfs:label xml:lang="en">constraint</rdfs:label>
        <rdfs:label xml:lang="fr">contrainte</rdfs:label>
        <rdfs:isDefinedBy rdf:resource="https://data.istex.fr/ontology/istex#"/>
    </owl:DatatypeProperty>
    
     <!-- https://data.istex.fr/ontology/istex#eISBN -->

    <owl:DatatypeProperty rdf:about="https://data.istex.fr/ontology/istex#eISBN">
        <rdfs:subPropertyOf rdf:resource="http://purl.org/ontology/bibo/identifier"/>
        <rdfs:domain rdf:resource="http://purl.org/ontology/bibo/Document"/>
        <rdfs:range rdf:resource="http://www.w3.org/2000/01/rdf-schema#Literal"/>
        <rdfs:comment xml:lang="fr">Identifiant électronique ISBN de l'objet documentaire.</rdfs:comment>
        <rdfs:comment xml:lang="en">The eISBN (electronic identifier) of the document.</rdfs:comment>
        <rdfs:label xml:lang="en">eISBN</rdfs:label>
        <rdfs:label xml:lang="fr">eISBN</rdfs:label>
        <rdfs:isDefinedBy rdf:resource="https://data.istex.fr/ontology/istex#"/>
    </owl:DatatypeProperty>


    <!-- https://data.istex.fr/ontology/istex#enrichmentType -->

    <owl:DatatypeProperty rdf:about="https://data.istex.fr/ontology/istex#enrichmentType">
        <rdfs:domain rdf:resource="https://data.istex.fr/ontology/istex#EnrichmentProcessConcept"/>
        <rdfs:range rdf:resource="http://www.w3.org/2000/01/rdf-schema#Literal"/>
        <rdfs:comment xml:lang="fr">Indique le type d'enrichissement créé.</rdfs:comment>
        <rdfs:comment xml:lang="en">Indicates the type of enrichment created.</rdfs:comment>
        <rdfs:label xml:lang="en">enrichment type</rdfs:label>
        <rdfs:label xml:lang="fr">type d'enrichissement</rdfs:label>
        <rdfs:isDefinedBy rdf:resource="https://data.istex.fr/ontology/istex#"/>
    </owl:DatatypeProperty>
    
    
     <!-- https://data.istex.fr/ontology/istex:identityProvider -->

    <owl:DatatypeProperty rdf:about="https://data.istex.fr/ontology/istex#identityProvider">
        <rdfs:domain rdf:resource="https://data.istex.fr/ontology/istex#Vocabulary"/>
        <rdfs:range rdf:resource="http://www.w3.org/2000/01/rdf-schema#Literal"/>
        <rdfs:comment xml:lang="fr">Indique le nom du fournisseur d'identité pour le vocabulaire "organization-list"</rdfs:comment>
        <rdfs:comment xml:lang="en">Specifies the name of the identity provider for the "organization-list" vocabulary</rdfs:comment>
        <rdfs:label xml:lang="en">identity provider</rdfs:label>
        <rdfs:label xml:lang="fr">fournisseur d'identité</rdfs:label>
        <rdfs:isDefinedBy rdf:resource="https://data.istex.fr/ontology/istex#"/>
    </owl:DatatypeProperty>


    <!-- https://data.istex.fr/ontology/istex#idIstex -->

    <owl:DatatypeProperty rdf:about="https://data.istex.fr/ontology/istex#idIstex">
        <rdfs:subPropertyOf rdf:resource="http://purl.org/ontology/bibo/identifier"/>
        <rdfs:domain rdf:resource="http://purl.org/ontology/bibo/Document"/>
        <rdfs:range rdf:resource="http://www.w3.org/2001/XMLSchema#anyURI"/>
        <rdfs:comment xml:lang="fr">Identifiant Istex de l'objet documentaire.</rdfs:comment>
        <rdfs:comment xml:lang="en">Istex identifier of the document object.</rdfs:comment>
        <rdfs:label xml:lang="en">Istex ident</rdfs:label>
        <rdfs:label xml:lang="fr">Identifiant Istex</rdfs:label>
        <rdfs:isDefinedBy rdf:resource="https://data.istex.fr/ontology/istex#"/>
    </owl:DatatypeProperty>
    
    
    <!-- https://data.istex.fr/ontology/istex#publicationTitle -->

    <owl:DatatypeProperty rdf:about="https://data.istex.fr/ontology/istex#publicationTitle">
        <rdfs:domain rdf:resource="http://purl.org/ontology/bibo/Document"/>
        <rdfs:range rdf:resource="http://www.w3.org/2000/01/rdf-schema#Literal"/>
        <rdfs:comment xml:lang="fr">Indique le titre du périodique hébergeant le document</rdfs:comment>
        <rdfs:comment xml:lang="en">Indicate the title of the periodical hosted the document</rdfs:comment>
        <rdfs:label xml:lang="en">publication title</rdfs:label>
        <rdfs:label xml:lang="fr">titre de la publication</rdfs:label>
        <rdfs:isDefinedBy rdf:resource="https://data.istex.fr/ontology/istex#"/>
    </owl:DatatypeProperty>
    

    <!-- https://data.istex.fr/ontology/istex#quantityOfItems -->

    <owl:DatatypeProperty rdf:about="https://data.istex.fr/ontology/istex#quantityOfItems">
        <rdfs:domain rdf:resource="http://www.w3.org/ns/dcat#Dataset"/>
        <rdfs:range rdf:resource="http://www.w3.org/2000/01/rdf-schema#Literal"/>
        <rdfs:comment xml:lang="fr">Indique le nombre de titres bibliographiques par corpus ISTEX</rdfs:comment>
        <rdfs:comment xml:lang="en">Indicates the number of bibliographic titles per ISTEX corpus</rdfs:comment>
        <rdfs:label xml:lang="fr">nombre de titres</rdfs:label>
        <rdfs:label xml:lang="en">number of titles</rdfs:label>
        <rdfs:isDefinedBy rdf:resource="https://data.istex.fr/ontology/istex#"/>
    </owl:DatatypeProperty>
    

    <!-- https://data.istex.fr/ontology/istex#query -->

    <owl:DatatypeProperty rdf:about="https://data.istex.fr/ontology/istex#query">
        <rdfs:domain rdf:resource="https://data.istex.fr/ontology/istex#Vocabulary"/>
        <rdfs:range rdf:resource="http://www.w3.org/2000/01/rdf-schema#Literal"/>
        <rdfs:comment xml:lang="fr">Indique la requête (API) à réaliser pour accéder aux documents indexés par le concept décrit. Cette API permet de récupérer les documents et le nombre de documents. Préfixer la requête avec "https://api.istex.fr/document/?q="" pour activer l'API.</rdfs:comment>
        <rdfs:comment xml:lang="en">Indicates the request (API) to make to access the documents indexed by the described concept. This API allows you to retrieve the documents and the number of documents. Prefix the query with "https: //api.istex.fr/document/?q=" to enable the API.</rdfs:comment>
        <rdfs:label xml:lang="en">query</rdfs:label>
        <rdfs:label xml:lang="fr">requête</rdfs:label>
        <rdfs:isDefinedBy rdf:resource="https://data.istex.fr/ontology/istex#"/>
    </owl:DatatypeProperty>
   
   <!-- https://data.istex.fr/ontology/istex#tool -->

    <owl:DatatypeProperty rdf:about="https://data.istex.fr/ontology/istex#tool">
        <rdfs:domain rdf:resource="https://data.istex.fr/ontology/istex#Vocabulary"/>
        <rdfs:range rdf:resource="http://www.w3.org/2000/01/rdf-schema#Literal"/>
        <rdfs:comment xml:lang="fr">Indique le nom de l'outil utilisé dans les processus d'enrichissement d'ISTEX</rdfs:comment>
        <rdfs:comment xml:lang="en">Specifies the name of the tool used in ISTEX enrichment processes</rdfs:comment>
        <rdfs:label xml:lang="en">software tool</rdfs:label>
        <rdfs:label xml:lang="fr">outil logiciel</rdfs:label>
        <rdfs:isDefinedBy rdf:resource="https://data.istex.fr/ontology/istex#"/>
    </owl:DatatypeProperty>

    <!-- 
    ///////////////////////////////////////////////////////////////////////////////////////
    //
    // Classes
    //
    ///////////////////////////////////////////////////////////////////////////////////////
     -->

    


    <!-- http://purl.org/dc/terms/LinguisticSystem -->

    <owl:Class rdf:about="http://purl.org/dc/terms/LinguisticSystem">
        <rdfs:subClassOf rdf:resource="http://www.w3.org/2004/02/skos/core#Concept"/>
        <rdfs:comment xml:lang="en">A system of signs, symbols, sounds, gestures, or rules used in communication.</rdfs:comment>
        <rdfs:label xml:lang="en">Linguistic System</rdfs:label>
    </owl:Class>
    


    <!-- http://purl.org/dc/terms/Location -->

    <owl:Class rdf:about="http://purl.org/dc/terms/Location">
        <rdfs:comment xml:lang="en">A spatial region or named place.</rdfs:comment>
        <rdfs:label xml:lang="en">Location</rdfs:label>
    </owl:Class>
    


    <!-- http://purl.org/dc/terms/PeriodOfTime -->

    <owl:Class rdf:about="http://purl.org/dc/terms/PeriodOfTime">
        <rdfs:comment xml:lang="en">An interval of time that is named or defined by its start and end dates.</rdfs:comment>
        <rdfs:label xml:lang="en">Period of Time</rdfs:label>
    </owl:Class>
    


    <!-- http://purl.org/ontology/bibo/Document -->

    <owl:Class rdf:about="http://purl.org/ontology/bibo/Document">
        <rdfs:subClassOf>
            <owl:Restriction>
                <owl:onProperty rdf:resource="http://purl.org/dc/terms/language"/>
                <owl:someValuesFrom rdf:resource="http://purl.org/dc/terms/LinguisticSystem"/>
            </owl:Restriction>
        </rdfs:subClassOf>
        <rdfs:subClassOf>
            <owl:Restriction>
                <owl:onProperty rdf:resource="http://purl.org/dc/terms/type"/>
                <owl:someValuesFrom rdf:resource="https://data.istex.fr/ontology/istex#ContentTypeConcept"/>
            </owl:Restriction>
        </rdfs:subClassOf>
        <rdfs:label>document</rdfs:label>
    </owl:Class>
    


    <!-- https://data.istex.fr/ontology/istex#ContentTypeConcept -->

    <owl:Class rdf:about="https://data.istex.fr/ontology/istex#ContentTypeConcept">
        <rdfs:subClassOf rdf:resource="http://www.w3.org/2004/02/skos/core#Concept"/>
        <rdfs:comment xml:lang="fr">Décrit la structure conceptuelle des types de contenus représentés dans les documents ISTEX</rdfs:comment>
        <rdfs:comment xml:lang="en">Describes the conceptual structure of the types of content represented in ISTEX documents</rdfs:comment>
        <rdfs:label xml:lang="en">Content Type Concept</rdfs:label>
        <rdfs:label xml:lang="fr">Concept de type de contenu</rdfs:label>
        <rdfs:isDefinedBy rdf:resource="https://data.istex.fr/ontology/istex#"/>
    </owl:Class>
    


    <!-- https://data.istex.fr/ontology/istex#EnrichmentProcessConcept -->

    <owl:Class rdf:about="https://data.istex.fr/ontology/istex#EnrichmentProcessConcept">
        <rdfs:subClassOf rdf:resource="http://www.w3.org/2004/02/skos/core#Concept"/>
        <rdfs:comment xml:lang="fr">Décrit la structure conceptuelle des processus d'enrichissements des documents ISTEX</rdfs:comment>
        <rdfs:comment xml:lang="en">Describe the conceptual structure of enrichment processes of ISTEX documents</rdfs:comment>
        <rdfs:label xml:lang="en">Enrichment Process Concept</rdfs:label>
        <rdfs:label xml:lang="fr">Concept de processus d'enrichissement</rdfs:label>
        <rdfs:isDefinedBy rdf:resource="https://data.istex.fr/ontology/istex#"/>
    </owl:Class>
    


    <!-- https://data.istex.fr/ontology/istex#GeographicConcept -->

    <owl:Class rdf:about="https://data.istex.fr/ontology/istex#GeographicConcept">
        <rdfs:subClassOf rdf:resource="http://www.w3.org/2004/02/skos/core#Concept"/>
        <rdfs:comment xml:lang="fr">Décrit la structure conceptuelle des entités nommées de nature géographique référencées dans les documents ISTEX</rdfs:comment>
        <rdfs:comment xml:lang="en">Describe the conceptual structure of the geographical entities referenced in the ISTEX documents</rdfs:comment>
        <rdfs:label xml:lang="en">Geographic Concept</rdfs:label>
        <rdfs:label xml:lang="fr">Concept géographique</rdfs:label>
        <rdfs:isDefinedBy rdf:resource="https://data.istex.fr/ontology/istex#"/>
    </owl:Class>
    


    <!-- https://data.istex.fr/ontology/istex#InistConcept -->

    <owl:Class rdf:about="https://data.istex.fr/ontology/istex#InistConcept">
        <rdfs:subClassOf rdf:resource="http://www.w3.org/2004/02/skos/core#Concept"/>
        <rdfs:comment xml:lang="fr">Décrit la structure conceptuelle des codes de classement Inist (Bases de données Pascal et Francis)</rdfs:comment>
        <rdfs:comment xml:lang="en">Describes the conceptual structure of Inist classification codes (database Pascal and Francis)</rdfs:comment>
        <rdfs:label xml:lang="en">Inist Concept</rdfs:label>
        <rdfs:label xml:lang="fr">Concept Inist</rdfs:label>
        <rdfs:isDefinedBy rdf:resource="https://data.istex.fr/ontology/istex#"/>
    </owl:Class>
    


    <!-- https://data.istex.fr/ontology/istex#NamedEntityConcept -->

    <owl:Class rdf:about="https://data.istex.fr/ontology/istex#NamedEntityConcept">
        <rdfs:subClassOf rdf:resource="http://www.w3.org/2004/02/skos/core#Concept"/>
        <rdfs:comment xml:lang="fr">Décrit la structure conceptuelle des entités nommées en général répertoriées dans les documents ISTEX</rdfs:comment>
        <rdfs:comment xml:lang="en">Describes the conceptual structure of named entities usually listed in ISTEX documents</rdfs:comment>
        <rdfs:label xml:lang="en">Named Entity Concept</rdfs:label>
        <rdfs:label xml:lang="fr">Concept d'entité nommée</rdfs:label>
        <rdfs:isDefinedBy rdf:resource="https://data.istex.fr/ontology/istex#"/>
    </owl:Class>
    


    <!-- https://data.istex.fr/ontology/istex#OrganizationConcept -->

    <owl:Class rdf:about="https://data.istex.fr/ontology/istex#OrganizationConcept">
        <rdfs:subClassOf rdf:resource="http://www.w3.org/2004/02/skos/core#Concept"/>
        <rdfs:comment xml:lang="fr">Décrit la structure conceptuelle des types d'organisations</rdfs:comment>
        <rdfs:comment xml:lang="en">Describe the conceptual structure of types of organizations</rdfs:comment>
        <rdfs:label xml:lang="en">Organization Concept</rdfs:label>
        <rdfs:label xml:lang="fr">Concept d'organisation</rdfs:label>
        <rdfs:isDefinedBy rdf:resource="https://data.istex.fr/ontology/istex#"/>
    </owl:Class>
    


    <!-- https://data.istex.fr/ontology/istex#PlaceConcept -->

    <owl:Class rdf:about="https://data.istex.fr/ontology/istex#PlaceConcept">
        <rdfs:subClassOf rdf:resource="http://www.w3.org/2004/02/skos/core#Concept"/>
        <rdfs:comment xml:lang="fr">Décrit la structure conceptuelle des entités nommées de type lieux référencées dans les documents ISTEX</rdfs:comment>
        <rdfs:comment xml:lang="en">Describes the conceptual structure of place-named entities referenced in ISTEX documents</rdfs:comment>
        <rdfs:label xml:lang="en">Place Concept</rdfs:label>
        <rdfs:label xml:lang="fr">Concept de lieu</rdfs:label>
        <rdfs:isDefinedBy rdf:resource="https://data.istex.fr/ontology/istex#"/>
    </owl:Class>
    


    <!-- https://data.istex.fr/ontology/istex#PublicationTypeConcept -->

    <owl:Class rdf:about="https://data.istex.fr/ontology/istex#PublicationTypeConcept">
        <rdfs:subClassOf rdf:resource="http://www.w3.org/2004/02/skos/core#Concept"/>
        <rdfs:comment xml:lang="fr">Décrit la structure conceptuelle des types de publication représentés dans les documents ISTEX</rdfs:comment>
        <rdfs:comment xml:lang="en">Describes the conceptual structure of the publication types represented in the ISTEX documents</rdfs:comment>
        <rdfs:label xml:lang="en">Publication Type Concept</rdfs:label>
        <rdfs:label xml:lang="fr">Concept type de publication</rdfs:label>
        <rdfs:isDefinedBy rdf:resource="https://data.istex.fr/ontology/istex#"/>
    </owl:Class>
    


    <!-- https://data.istex.fr/ontology/istex#PublisherConcept -->

    <owl:Class rdf:about="https://data.istex.fr/ontology/istex#PublisherConcept">
        <rdfs:subClassOf rdf:resource="http://www.w3.org/2004/02/skos/core#Concept"/>
        <rdfs:comment xml:lang="fr">Décrit la structure conceptuelle des éditeurs (publishers) en lien avec les documents ISTEX</rdfs:comment>
        <rdfs:comment xml:lang="en">Describes the publishers' conceptual structure in relation to ISTEX documents</rdfs:comment>
        <rdfs:label xml:lang="en">Publisher Concept</rdfs:label>
        <rdfs:label xml:lang="fr">Concept Editeur</rdfs:label>
        <rdfs:isDefinedBy rdf:resource="https://data.istex.fr/ontology/istex#"/>
    </owl:Class>
    


    <!-- https://data.istex.fr/ontology/istex#ScienceMetrixConcept -->

    <owl:Class rdf:about="https://data.istex.fr/ontology/istex#ScienceMetrixConcept">
        <rdfs:subClassOf rdf:resource="http://www.w3.org/2004/02/skos/core#Concept"/>
        <rdfs:comment xml:lang="fr">Décrit la structure conceptuelle des catégories Science Metrix</rdfs:comment>
        <rdfs:comment xml:lang="en">Describes the conceptual structure of the Science Metrix categories</rdfs:comment>
        <rdfs:label xml:lang="en">Science Metrix Concept</rdfs:label>
        <rdfs:label xml:lang="fr">Concept Science Metrix</rdfs:label>
        <rdfs:isDefinedBy rdf:resource="https://data.istex.fr/ontology/istex#"/>
    </owl:Class>

    
    
    <!-- https://data.istex.fr/ontology/istex#ScientificDomain -->

    <owl:Class rdf:about="https://data.istex.fr/ontology/istex#ScientificDomain">
        <rdfs:subClassOf rdf:resource="http://www.w3.org/2004/02/skos/core#Concept"/>
        <rdfs:comment xml:lang="fr">Décrit les domaines scientifiques présents sur le site licence nationale.</rdfs:comment>
        <rdfs:comment xml:lang="en">Describes the scientific fields present on the national license site.</rdfs:comment>
        <rdfs:label xml:lang="en">Scientific Domain</rdfs:label>
        <rdfs:label xml:lang="fr">Domaine scientifique</rdfs:label>
        <rdfs:isDefinedBy rdf:resource="https://data.istex.fr/ontology/istex#"/>
    </owl:Class>
    
    <!-- https://data.istex.fr/ontology/istex#ScopusConcept -->
    
    <owl:Class rdf:about="https://data.istex.fr/ontology/istex#ScopusConcept">
        <rdfs:subClassOf rdf:resource="http://www.w3.org/2004/02/skos/core#Concept"/>
        <rdfs:comment xml:lang="fr">Décrit la structure conceptuelle des catégories Scopus</rdfs:comment>
        <rdfs:comment xml:lang="en">Describes the conceptual structure of the Scopus categories</rdfs:comment>
        <rdfs:label xml:lang="en">Scopus Concept</rdfs:label>
        <rdfs:label xml:lang="fr">Concept Scopus</rdfs:label>
        <rdfs:isDefinedBy rdf:resource="https://data.istex.fr/ontology/istex#"/>
    </owl:Class>
    
    
    <!-- https://data.istex.fr/ontology/istex#Vocabulary -->
    
    <owl:Class rdf:about="https://data.istex.fr/ontology/istex#Vocabulary">
        <rdfs:subClassOf rdf:resource="http://rdfs.org/ns/void#Dataset"/>
        <rdfs:subClassOf rdf:resource="http://purl.org/vocab/frbr/core#Work"/>
        <rdfs:comment xml:lang="fr">Décrit les vocabulaires utilisés dans l'ontologie ISTEX</rdfs:comment>
        <rdfs:comment xml:lang="en">Describes ISTEX' vocabularies</rdfs:comment>
        <rdfs:label xml:lang="en">Vocabulary</rdfs:label>
        <rdfs:label xml:lang="fr">Vocabulaire</rdfs:label>
        <rdfs:isDefinedBy rdf:resource="https://data.istex.fr/ontology/istex#"/>
    </owl:Class>
    
    <!-- https://data.istex.fr/ontology/istex#WosConcept -->
    
    <owl:Class rdf:about="https://data.istex.fr/ontology/istex#WosConcept">
        <rdfs:subClassOf rdf:resource="http://www.w3.org/2004/02/skos/core#Concept"/>
        <rdfs:comment xml:lang="fr">Décrit la structure conceptuelle des catégories Web of Science</rdfs:comment>
        <rdfs:comment xml:lang="en">Describes the conceptual structure of the Web of Science categories</rdfs:comment>
        <rdfs:label xml:lang="en">Web Of Science Concept</rdfs:label>
        <rdfs:label xml:lang="fr">Concept Web Of Science</rdfs:label>
        <rdfs:isDefinedBy rdf:resource="https://data.istex.fr/ontology/istex#"/>
    </owl:Class>
</rdf:RDF>



<!-- Generated by the OWL API (version 4.2.6.20160910-2108) https://github.com/owlcs/owlapi -->

